extraction: Prove a generalized loop lemma

src/CertifiedExtraction/ADTExamples.v
@@ -6,7 +6,7 @@ Require Import
         CertifiedExtraction.Extraction.AllInternal
         CertifiedExtraction.Extraction.Extraction.
 
-Definition MyEnvLists :=
+Definition MyEnvLists `{FacadeWrapper av (list W)} :=
   (GLabelMap.add ("std", "rand") (Axiomatic FRandom))
     ((GLabelMap.add ("list", "nil") (Axiomatic (FacadeImplementationOfConstructor nil)))
        ((GLabelMap.add ("list", "push") (Axiomatic (FacadeImplementationOfMutation cons)))
@@ -15,7 +15,7 @@ Definition MyEnvLists :=
                 ((GLabelMap.add ("list", "empty?") (Axiomatic List_empty))
                    (GLabelMap.empty (FuncSpec (list W)))))))).
 
-Example other_test_with_adt'' :
+Example other_test_with_adt'' `{FacadeWrapper av (list W)}:
     sigT (fun prog => forall seq: list W, {{ [["arg1" <-- seq as _ ]] :: Nil }}
                                     prog
                                   {{ [["ret" <-- (List.fold_left (@Word.wminus 32) seq 0) as _]] :: Nil }} ∪ {{ StringMap.empty _ }} // MyEnvLists).
@@ -35,34 +35,108 @@ Eval compute in (extract_facade other_test_with_adt'').
 
 Eval cbv beta iota zeta delta [extract_facade Fold proj1_sig sig_of_sigT other_test_with_adt'' WrapOpInExpr] in (extract_facade other_test_with_adt'').
 
-Definition fold_comp {TAcc TElem} (f: TAcc -> TElem -> Comp TAcc) seq init :=
-  List.fold_left (fun acc elem =>
-                    ( acc <- acc;
-                      f acc elem )%comp)
-                 seq (ret init).
+Definition fold_comp {TAcc TElem} (f: Comp TAcc -> TElem -> Comp TAcc) seq init :=
+  List.fold_left (fun (acc: Comp TAcc) (elem: TElem) =>
+                    ( f acc elem )%comp)
+                 seq init.
 
-Example other_test_with_adt''' `{FacadeWrapper (Value (list W)) (list W)} f:
+Require Import
+        CertifiedExtraction.Extraction.AllInternal
+        CertifiedExtraction.Extraction.External.Core
+        CertifiedExtraction.Extraction.External.Loops
+        CertifiedExtraction.Extraction.External.GenericADTMethods
+        CertifiedExtraction.Extraction.External.FacadeADTs.
+
+(* Opaque WrapInstance.            (* FIXME simpl never? *) *)
+
+Lemma CompileLoop :
+  forall `{FacadeWrapper av (list W)}
+    lst init vhead vtest vlst vret fpop fempty fdealloc facadeInit facadeBody env (ext: StringMap.t (Value av)) tenv (f: Comp W -> W -> Comp W),
+    GLabelMap.MapsTo fpop (Axiomatic List_pop) env ->
+    GLabelMap.MapsTo fempty (Axiomatic List_empty) env ->
+    GLabelMap.MapsTo fdealloc (Axiomatic (FacadeImplementationOfDestructor (A := list W))) env ->
+    vtest ∉ ext ->
+    NotInTelescope vtest tenv ->
+    vlst ∉ ext ->
+    NotInTelescope vlst tenv ->
+    vret ∉ ext ->
+    NotInTelescope vret tenv ->
+    vhead ∉ ext ->
+    NotInTelescope vhead tenv ->
+    vtest <> vret ->
+    vtest <> vlst ->
+    vtest <> vhead ->
+    vret <> vlst ->
+    vret <> vhead ->
+    vlst <> vhead ->
+    {{ [[`vlst <~~ lst as _]] :: tenv }}
+      facadeInit
+    {{ [[`vret <~~ init as _]] :: [[`vlst <~~ lst as _]] :: tenv }} ∪ {{ ext }} // env ->
+    (forall head (acc: Comp W) (s: Comp (list W)),
+        {{ [[vhead <-- head as _]] :: [[`vlst <~~ s as _]] :: [[vtest <-- (bool2w false) as _]] :: [[`vret <~~ acc as _]] :: tenv }}
+          facadeBody
+        {{ [[`vlst <~~ s as _]] :: [[vtest <-- (bool2w false) as _]] :: [[`vret <~~ (f acc head) as _]] :: tenv }} ∪ {{ ext }} // env) ->
+    {{ [[`vlst <~~ lst as _]] :: tenv }}
+      (Seq facadeInit (Seq (Fold vhead vtest vlst fpop fempty facadeBody) (Call vtest fdealloc (vlst :: nil))))
+    {{ [[lst as ls]] :: [[`vret <~~ (fold_comp f ls init) as _]] :: tenv }} ∪ {{ ext }} // env.
+Proof.
+  Require Import FacadeLoops.
+  loop_t.
+
+  rewrite TelEq_swap by congruence;
+    eapply CompileCallEmpty_spec; loop_t.
+
+  2:eapply CompileCallFacadeImplementationOfDestructor; loop_t.
+
+  rewrite (TelEq_swap (k' := None)) by loop_t.
+
+  apply miniChomp'; loop_t.
+
+  clear dependent facadeInit;
+  generalize dependent init;
+  generalize dependent lst;
+  induction vv; loop_t.
+
+  rewrite TelEq_swap by loop_t.
+
+  apply CompileWhileFalse_Loop; loop_t.
+
+  eapply CompileWhileTrue; loop_t.
+
+  apply generalized CompileCallPop; loop_t.
+
+  apply CompileCallEmpty_spec; loop_t.
+
+  loop_t.
+Qed.
+
+Example other_test_with_adt''' `{FacadeWrapper av (list W)} f:
     sigT (fun prog => {{ Nil }}
                      prog
                    {{ [[`"ret" <~~  ( seq <- {s: list W | True };
-                                    res <- fold_comp f seq (Word.natToWord 32 0: W);
-                                    ret res) as _]] :: Nil }} ∪ {{ StringMap.empty _ }} // MyEnvLists).
+                                    fold_comp f seq (ret (Word.natToWord 32 0: W))) as _]] :: Nil }} ∪ {{ StringMap.empty _ }} // MyEnvLists).
 Proof.
   econstructor; intros.
 
   repeat setoid_rewrite SameValues_Fiat_Bind_TelEq.
+
   eapply ProgOk_Transitivity_Name' with "seq".
 
   Focus 2.
 
-  Require Import QueryStructure.Specification.Operations.FlattenCompList.
-  Check flatten_CompList.
+  let av := av_from_ext (StringMap.empty (Value (list W))) in
+  let fpop := find_function_pattern_in_env
+               (fun w => (Axiomatic (List_pop (av := av) (H := w)))) MyEnvLists in
+  let fempty := find_function_pattern_in_env
+                 (fun w => (Axiomatic (List_empty (av := av) (H := w)))) MyEnvLists in
+  let fdealloc := find_function_pattern_in_env
+                   (fun w => (Axiomatic (FacadeImplementationOfDestructor
+                                        (A := list W) (av := av) (H := w)))) MyEnvLists in
+  let vtest := gensym "test" in
+  let vhead := gensym "head" in
+  apply (CompileLoop (vtest := vtest) (vhead := vhead) (fpop := fpop) (fempty := fempty) (fdealloc := fdealloc)); try compile_do_side_conditions; repeat compile_step.
 
-  repeat (compile_step || compile_loop).
-  let fop := translate_op Word.wminus in
-  apply (CompileBinopOrTest_right_inPlace fop); compile_do_side_conditions.
 Defined.
-
 
 Example other_test_with_adt'' :
     sigT (fun prog => forall seq seq', {{ [["arg1" <-- seq as _ ]] :: [["arg2" <-- seq' as _]] :: Nil }}
