src/CertifiedExtraction/Extraction/External/FacadeADTs.v
@@ -32,41 +32,6 @@ Lemma CompileCallEmpty:
     (fempty : GLabelMap.key) (lst : list W),
     vlst <> vtest ->
     vtest ∉ ext ->
-    NotInTelescope vtest tenv ->
-    vlst ∉ ext ->
-    NotInTelescope vlst tenv ->
-    GLabelMap.MapsTo fempty (Axiomatic List_empty) env ->
-    {{ [[vlst <-- lst as _]]::tenv }}
-      Call vtest fempty (vlst :: nil)
-    {{ [[vtest <-- (bool2w match lst with
-                         | nil => true
-                         | _ :: _ => false
-                         end) as _]]::[[vlst <-- lst as _]]::tenv }} ∪ {{ ext }} // env.
-Proof.
-  repeat match goal with
-         | _ => SameValues_Facade_t_step
-         | _ => facade_cleanup_call
-         (* | [ H: ADT _ = ADT _ |- _ ] => inversion' H *)
-         (* | [  |- context[wrap (FacadeWrapper := WrapInstance) ?x]     ] => rewrite WrapInstance_wrap *)
-         (* | [ H: context[wrap (FacadeWrapper := WrapInstance) _] |- _ ] => rewrite WrapInstance_wrap in H *)
-         (* | _ => rewrite WrapInstance_unwrap_wrap *)
-         end.
-
-  facade_eauto.
-  facade_eauto.
-  facade_eauto.
-  facade_eauto.
-
-  eapply (SameValues_PopExt' (H := WrapInstance (H := H))). (* FIXME *)
-  facade_eauto.
-  facade_eauto.
-Qed.
-
-Lemma CompileCallEmpty':
-  forall `{FacadeWrapper av (list W)} (vtest vlst : StringMap.key) (env : GLabelMap.t (FuncSpec av)) (tenv: Telescope av) ext
-    (fempty : GLabelMap.key) (lst : list W),
-    vlst <> vtest ->
-    vtest ∉ ext ->
     Lifted_MapsTo ext tenv vlst (wrap lst) ->
     Lifted_not_mapsto_adt ext tenv vtest ->
     GLabelMap.MapsTo fempty (Axiomatic List_empty) env ->
@@ -77,9 +42,8 @@ Lemma CompileCallEmpty':
                          | _ :: _ => false
                          end) as _]]::(DropName vtest tenv) }} ∪ {{ ext }} // env.
 Proof.
-  repeat match goal with
-         | _ =>  SameValues_Facade_t_step || facade_cleanup_call || LiftPropertyToTelescope_t
-         end.
+  repeat (SameValues_Facade_t_step || facade_cleanup_call || LiftPropertyToTelescope_t).
+  facade_eauto.
   facade_eauto.
   facade_eauto.
   rewrite <- remove_add_comm by congruence. (* FIXME *)
@@ -88,7 +52,60 @@ Proof.
   rewrite <- add_redundant_cancel; eauto.
 Qed.
 
-Lemma CompileCallPop':
+(* Lemma CompileCallEmpty: *)
+(*   forall `{FacadeWrapper av (list W)} (vtest vlst : StringMap.key) (env : GLabelMap.t (FuncSpec av)) (tenv: Telescope av) ext *)
+(*     (fempty : GLabelMap.key) (lst : list W), *)
+(*     vlst <> vtest -> *)
+(*     vtest ∉ ext -> *)
+(*     NotInTelescope vtest tenv -> *)
+(*     vlst ∉ ext -> *)
+(*     NotInTelescope vlst tenv -> *)
+(*     GLabelMap.MapsTo fempty (Axiomatic List_empty) env -> *)
+(*     {{ [[vlst <-- lst as _]]::tenv }} *)
+(*       Call vtest fempty (vlst :: nil) *)
+(*     {{ [[vtest <-- (bool2w match lst with *)
+(*                          | nil => true *)
+(*                          | _ :: _ => false *)
+(*                          end) as _]]::[[vlst <-- lst as _]]::tenv }} ∪ {{ ext }} // env. *)
+(* Proof. *)
+(*   repeat match goal with *)
+(*          | _ => SameValues_Facade_t_step *)
+(*          | _ => facade_cleanup_call *)
+(*          (* | [ H: ADT _ = ADT _ |- _ ] => inversion' H *) *)
+(*          (* | [  |- context[wrap (FacadeWrapper := WrapInstance) ?x]     ] => rewrite WrapInstance_wrap *) *)
+(*          (* | [ H: context[wrap (FacadeWrapper := WrapInstance) _] |- _ ] => rewrite WrapInstance_wrap in H *) *)
+(*          (* | _ => rewrite WrapInstance_unwrap_wrap *) *)
+(*          end. *)
+
+(*   facade_eauto. *)
+(*   facade_eauto. *)
+(*   facade_eauto. *)
+(*   facade_eauto. *)
+
+(*   eapply (SameValues_PopExt' (H := WrapInstance (H := H))). (* FIXME *) *)
+(*   facade_eauto. *)
+(*   facade_eauto. *)
+(* Qed. *)
+
+Lemma CompileCallEmpty_spec:
+  forall `{FacadeWrapper av (list W)} (vtest vlst : StringMap.key) (env : GLabelMap.t (FuncSpec av)) (tenv: Telescope av) ext
+    (fempty : GLabelMap.key) (lst : Comp (list W)),
+    vlst <> vtest ->
+    vtest ∉ ext ->
+    Lifted_not_mapsto_adt ext tenv vtest ->
+    GLabelMap.MapsTo fempty (Axiomatic List_empty) env ->
+    {{ [[`vlst <~~ lst as _]] :: tenv }}
+      Call vtest fempty (vlst :: nil)
+    {{ [[`vlst <~~ lst as ls]] :: [[vtest <-- (bool2w match ls with
+                                                | nil => true
+                                                | _ :: _ => false
+                                                end) as _]] :: (DropName vtest tenv) }} ∪ {{ ext }} // env.
+Proof.
+  repeat (SameValues_Facade_t_step || facade_cleanup_call || LiftPropertyToTelescope_t);
+  facade_eauto.
+Qed.
+
+Lemma CompileCallPop:
   forall `{FacadeWrapper av (list W)} (vhead vlst : StringMap.key) (env : GLabelMap.t (FuncSpec av)) tenv ext
     (fpop : GLabelMap.key) head (tail : list W),
     vlst <> vhead ->
